theories/c_lang/derived_laws.v
@@ -15,6 +15,7 @@ From iris.prelude Require Import options.
 lead to overlapping instances. *)
 
 Section lifting.
+Context {SI:indexT}.
 Context `{!heapG_C Σ, !invG Σ}.
 Context {p:program}.
 Implicit Types P Q : iProp Σ.
